compiler/dafny/vcg/dafny_vcg_exampleScript.sml
@@ -1,0 +1,192 @@
+(*
+  Concrete examples demonstrating the wp calculus.
+*)
+Theory dafny_vcg_example
+Ancestors
+  dafny_semanticPrimitives
+  dafny_evaluate
+  dafny_eval_rel
+  dafny_freshen
+  dafny_wp_calc
+Libs
+  preamble
+
+(* Stop EVAL from deep-frying the statement in valid_vcg_prop *)
+val _ = computeLib.del_funs [forall_def, eval_true_def];
+
+(* Freshen pass: Make variable names unique and start with v *)
+fun eval_freshen prog = EVAL “freshen_program $ ^prog” |> concl |> rhs;
+
+(* Generate VCG for all methods *)
+fun eval_vcg prog = EVAL “vcg ^prog” |> concl |> rhs |> rand;
+
+(* Quantify over the given (free) variables, and turn the list of conditions
+   into a single condition using conjunction *)
+Definition list_to_conj_def:
+  list_to_conj [] = T ∧
+  list_to_conj (x::xs) = (x ∧ list_to_conj xs)
+End
+
+fun valid_vcg_prop vcgs =
+  EVAL “list_to_conj $ MAP (λ(var,prop). forall var prop) ^vcgs” |> concl |> rhs;
+
+(** Example 1: Adding one to an integer ensures that it is strictly larger ****)
+
+val plus_one = eval_freshen
+  “Program
+   [Method «PlusOne» [(«n»,IntT)] [] [int_lt (Var «n») (Var «r»)] []
+     [Var «n»] [(«r»,IntT)] []
+     (Then
+        (Assign [(VarLhs «r»,ExpRhs (BinOp Add (Var «n») (int_lit 1)))])
+        Return)]”;
+
+
+val plus_one_vcg = eval_vcg plus_one;
+
+val plus_one_valid_prop = valid_vcg_prop plus_one_vcg;
+
+(* Unrolls a few definitions to make a bit of progress. *)
+fun step n =
+  simp [Ntimes evaluate_exp_def n, read_local_def, do_sc_def, do_bop_def,
+        push_locals_def, pop_locals_def, safe_drop_def, use_old_def,
+        unuse_old_def, do_cond_def, get_locs_def, do_uop_def, get_array_len_def,
+        index_array_def, val_to_num_def,
+        dafny_semanticPrimitivesTheory.get_loc_def, push_local_def];
+
+Theorem plus_one_correct:
+  ^plus_one_valid_prop
+Proof
+  simp [forall_def, strict_locals_ok_def, state_inv_def, eval_true_def,
+        eval_exp_def, all_values_def]
+  \\ rpt strip_tac
+  \\ ‘ALOOKUP st.locals_old «v0» = SOME (SOME val)’ by (gvs [])
+  \\ step 20
+  \\ simp [state_component_equality]
+QED
+
+(** Example 2: McCarthy's 91 function *****************************************)
+
+val mccarthy = eval_freshen
+  “Program
+     [Method «M» [(«n»,IntT)] []
+       [dfy_eq (Var «r»)
+          (If (int_le (Var «n») (int_lit 100)) (int_lit 91)
+             (BinOp Sub (Var «n») (int_lit 10)))] []
+       [BinOp Sub (int_lit 111) (Var «n»)] [(«r»,IntT)] []
+         (Then
+            (If (int_le (Var «n») (int_lit 100))
+               (Dec («tmp»,IntT)
+                  (Then
+                   (MetCall [VarLhs «tmp»] «M»
+                      [BinOp Add (Var «n») (int_lit 11)])
+                   (MetCall [VarLhs «r»] «M» [Var «tmp»])))
+               (Assign
+                  [(VarLhs «r»,ExpRhs (BinOp Sub (Var «n») (int_lit 10)))]))
+            Return)]”;
+
+val mccarthy_vcg = eval_vcg mccarthy;
+
+val mccarthy_valid_prop = valid_vcg_prop mccarthy_vcg;
+
+(* Make the goal actually readable *)
+val _ = max_print_depth := 20;
+
+Triviality eval_forall_True:
+  (∀v. v ∈ dom ⇒ SND (eval v) = Rval (BoolV T)) ⇒
+  eval_forall dom eval = Rval (BoolV T)
+Proof
+  rpt strip_tac
+  \\ gvs [eval_forall_def, AllCaseEqs()]
+  \\ rpt strip_tac \\ gvs []
+QED
+
+Theorem mccarthy_correct:
+  ^mccarthy_valid_prop
+Proof
+  (* TODO Combine simps; the main thing that probably needs some care is that
+     the parts around "qmatch_goalsub_abbrev_tac ‘eval_forall dom evalf’" keep
+     working. *)
+  simp [forall_def, strict_locals_ok_def, state_inv_def, eval_true_def,
+        eval_exp_def, all_values_def]
+  \\ rpt strip_tac
+  \\ ‘ALOOKUP st.locals_old «v0» = SOME (SOME val)’ by (gvs [])
+  \\ step 20
+  \\ IF_CASES_TAC \\ simp []
+  >- (* i > 100 *)
+   (step 40 \\ simp [state_component_equality])
+  \\ step 30
+  \\ IF_CASES_TAC \\ gvs [] >- (intLib.COOPER_TAC)
+  \\ step 20
+  \\ IF_CASES_TAC \\ gvs [] >- (intLib.COOPER_TAC)
+  \\ step 20
+  \\ IF_CASES_TAC \\ simp []
+  >- (spose_not_then kall_tac \\ intLib.COOPER_TAC)
+  \\ step 15
+  \\ IF_CASES_TAC \\ simp [] >- (intLib.COOPER_TAC)
+  \\ qexists ‘111’ \\ simp []
+  \\ qmatch_goalsub_abbrev_tac ‘eval_forall dom evalf’
+  \\ ‘eval_forall dom evalf = Rval (BoolV T)’ by
+    (irule eval_forall_True
+     \\ rpt strip_tac
+     \\ unabbrev_all_tac
+     \\ gvs [all_values_def]
+     \\ IF_CASES_TAC \\ simp []
+     >- (* ¬(i + 11 ≤ 100) *)
+      (step 10
+       \\ IF_CASES_TAC \\ simp []
+       \\ step 10
+       \\ IF_CASES_TAC \\ simp [] >- (intLib.COOPER_TAC)
+       \\ step 20
+       \\ IF_CASES_TAC \\ simp [] >- (spose_not_then kall_tac \\ intLib.COOPER_TAC)
+       \\ step 20
+       \\ IF_CASES_TAC \\ simp [] >- (intLib.COOPER_TAC)
+       \\ reverse IF_CASES_TAC \\ simp [] >- (intLib.COOPER_TAC)
+       \\ qmatch_goalsub_abbrev_tac ‘eval_forall dom evalf’
+       \\ ‘eval_forall dom evalf = Rval (BoolV T)’ by
+         (irule eval_forall_True
+          \\ rpt strip_tac
+          \\ unabbrev_all_tac
+          \\ gvs [all_values_def]
+          \\ step 30
+          \\ IF_CASES_TAC \\ simp [])
+       \\ simp []
+       \\ strip_tac >- (intLib.COOPER_TAC))
+     (* i + 11 ≤ 100 *)
+     \\ step 5
+     \\ gvs [value_same_type_def, all_values_def]
+     \\ simp [pop_locals_def, safe_drop_def]
+     \\ IF_CASES_TAC >- (simp [])
+     \\ step 20
+     \\ IF_CASES_TAC \\ simp [] >- (intLib.COOPER_TAC)
+     \\ step 20
+     \\ IF_CASES_TAC \\ simp [] >- (spose_not_then kall_tac \\ intLib.COOPER_TAC)
+     \\ step 20
+     \\ IF_CASES_TAC \\ simp [] >- (intLib.COOPER_TAC)
+     \\ reverse IF_CASES_TAC \\ simp [] >- (intLib.COOPER_TAC)
+     \\ qmatch_goalsub_abbrev_tac ‘eval_forall dom evalf’
+     \\ ‘eval_forall dom evalf = Rval (BoolV T)’ by
+       (irule eval_forall_True
+        \\ rpt strip_tac
+        \\ unabbrev_all_tac
+        \\ gvs [all_values_def]
+        \\ step 20
+        \\ IF_CASES_TAC \\ simp []
+          >- (* ≤ 100 *)
+           (step 5
+            \\ IF_CASES_TAC \\ simp []
+            \\ step 10
+            \\ IF_CASES_TAC \\ simp []
+            \\ IF_CASES_TAC \\ simp []
+            \\ intLib.COOPER_TAC)
+        \\ step 10
+        \\ IF_CASES_TAC \\ simp []
+        \\ IF_CASES_TAC \\ simp []
+        \\ intLib.COOPER_TAC)
+     \\ simp []
+     \\ intLib.COOPER_TAC)
+  (* ¬ ≤ 100*)
+  \\ step 20
+  \\ IF_CASES_TAC \\ simp []
+  \\ simp [state_component_equality]
+  \\ intLib.COOPER_TAC
+QED
